\begin{enumerate}
\item First observe that $1 - \P(y = y^{(i)}|\mathbf{x}^{(i)}) = \frac{\exp(-\bm{\theta}^\top \mathbf{x}^{(i)})}{1 + \exp(-\bm{\theta}^\top \mathbf{x}^{(i)})} = \frac{1}{1 + \exp(\bm{\theta}^\top \mathbf{x}^{(i)})} = \P(y = y^{(i)}|-\mathbf{x}^{(i)}).$ \\
With this we get that
$\log \left(\P(y = y^{(i)}|\mathbf{x}^{(i)})\right) = \log\left(\P(y = y^{(i)}|\mathbf{x}^{(i)})^{y^{(i)}}(1-\P(y = y^{(i)}|\mathbf{x}^{(i)})^{1-y^{(i)}}\right)$ \\
$\quad = y^{(i)}\log (\P(y = y^{(i)}|\mathbf{x}^{(i)})) + (1-y^{(i)})\log((1-\P(y = y^{(i)}|\mathbf{x}^{(i)})$ \\
$\quad = y^{(i)}(\log (\P(y = y^{(i)}|\mathbf{x}^{(i)})) - \log (\P(y = y^{(i)}|-\mathbf{x}^{(i)})) ) + \log(\P(y = y^{(i)}|-\mathbf{x}^{(i)}))$ \\
$\quad = y^{(i)}\left(\log\left(\frac{ \P(y = y^{(i)}|\mathbf{x}^{(i)})}{ \P(y = y^{(i)}|-\mathbf{x}^{(i)})}\right)\right) + \log(\P(y = y^{(i)}|-\mathbf{x}^{(i)}))$ \\
$\quad = y^{(i)}\left(\log\left(\frac{ 1 + \exp(\bm{\theta}^\top \mathbf{x}^{(i)})}{ 1 + \exp(-\bm{\theta}^\top \mathbf{x}^{(i)})}\right)\right) - \log(1 + \exp(\bm{\theta}^\top \mathbf{x}^{(i)}))$ \\
$\quad = y^{(i)}\left(\log\left(\exp(\bm{\theta}^\top \mathbf{x}^{(i)})\frac{ 1 + \exp(-\bm{\theta}^\top \mathbf{x}^{(i)})}{ 1 + \exp(-\bm{\theta}^\top \mathbf{x}^{(i)})}\right)\right) - \log(1 + \exp(\bm{\theta}^\top \mathbf{x}^{(i)}))$ \\
$\quad = y^{(i)}\bm{\theta}^\top \mathbf{x}^{(i)} - \log(1 + \exp(\bm{\theta}^\top \mathbf{x}^{(i)}))$ \\
With this we find that $\mathcal{R}_\text{emp} = -\log \prod^n_{i=1}\P(y = y^{(i)}|\mathbf{x}^{(i)}) = \sum^n_{i=1}y^{(i)} \log(1 + \exp(\bm{\theta}^\top \mathbf{x}^{(i)})) - y^{(i)}\bm{\theta}^\top \mathbf{x}^{(i)} $

\item $\frac{\partial}{\partial \bm{\theta}}\mathcal{R}_{\text{emp}} = \sum^n_{i=1}y^{(i)} \frac{\exp(\bm{\theta}^\top \mathbf{x}^{(i)})}{1 + \exp(\bm{\theta}^\top \mathbf{x}^{(i)})}{\mathbf{x}^{(i)}}^\top - y^{(i)}{\mathbf{x}^{(i)}}^\top$ \\
$\frac{\partial^2}{\partial \bm{\theta}\partial \bm{\theta}^\top}\mathcal{R}_{\text{emp}} = \sum^n_{i=1}y^{(i)} \frac{\exp(\bm{\theta}^\top \mathbf{x}^{(i)})(1 + \exp(\bm{\theta}^\top \mathbf{x}^{(i)}) - \exp(\bm{\theta}^\top \mathbf{x}^{(i)})^2}{(1 + \exp(\bm{\theta}^\top \mathbf{x}^{(i)})^2}\mathbf{x}^{(i)}{\mathbf{x}^{(i)}}^\top =  \sum^n_{i=1}\underbrace{y^{(i)} \frac{\exp(\bm{\theta}^\top \mathbf{x}^{(i)})}{(1 + \exp(\bm{\theta}^\top \mathbf{x}^{(i)})^2}}_{\geq 0}\underbrace{\mathbf{x}^{(i)}{\mathbf{x}^{(i)}}^\top}_{\text{p.s.d.}}$ \\
is p.s.d. $\Rightarrow \mathcal{R}_{\text{emp}}$ is convex.

\item We can transform the inequalities such that \\
$\zeta^{(i)} \geq 1 - y^{(i)}\left( \bm{\theta}^\top\mathbf{x}^{(i)} + \bm{\theta}_0\right) \quad \forall i \in \{1,\dots,n\}$ and $\zeta^{(i)} \geq 0 \quad \forall i \in \{1, \dots, n\}.$\\
We can find the smallest $\zeta^{(i)}$ by assuring that always at least one constraint is active:\\
$\zeta^{(i)} = \begin{cases} 1 - y^{(i)}\left( \bm{\theta}^\top\mathbf{x}^{(i)} + \bm{\theta}_0\right) & \text{for } 1 - y^{(i)}\left( \bm{\theta}^\top\mathbf{x}^{(i)} + \bm{\theta}_0\right) \geq 0 \\
0 & \text{for } 1 - y^{(i)}\left( \bm{\theta}^\top\mathbf{x}^{(i)} + \bm{\theta}_0\right) < 0
\end{cases} = \max(1 - y^{(i)}\left( \bm{\theta}^\top\mathbf{x}^{(i)} + \bm{\theta}_0\right), 0)$ \\
Inserting these $\zeta^{(i)}$ into the objective function results in $f(\bm{\theta}) =
\frac{1}{2}\Vert\bm{\theta}\Vert^2_2 + C\sum^n_{i=1}\max(1-y^{(i)}\bm{\theta}^\top\mathbf{x}^{(i)} + \bm{\theta}_0, 0).$
Minimzing $f$ is equivalent to minimizing $\frac{1}{2C}\Vert\bm{\theta}\Vert^2_2 + \sum^n_{i=1}\max(1-y^{(i)}\bm{\theta}^\top\mathbf{x}^{(i)} + \bm{\theta}_0, 0) \Rightarrow \lambda = \frac{1}{2C}.$

\item First we show that $g:\R \rightarrow \R, x \mapsto \max(x, 0)$ is convex: \\
Let $x, y \in R, t \in [0, 1]: g(x + t(y-x)) = \max(x + t(y-x), 0)$

\end{enumerate}
