\begin{enumerate}
\item Let $x,y \in \R$ and $t \in [0, 1]$ then it holds that
\begin{align*}
(f + g)(x + t(y-x)) &= f(x + t(y-x)) + g(x + t(y-x)) \\
&\leq f(x) + t(f(y)-f(x)) + g(x) + t(g(y)-g(x)) & \text{($f,g$ are convex)} \\
& = f(x) + g(x) + t(f(y) + g(y) -(f(x) + g(x))) \\
& = (f + g)(x) + t((f + g)(y) - (f + g)(x))
\end{align*}
\item Now, assume that g is additionally non-decreasing, i.e., $g(y) \geq g(x) \; \forall x \in \R, \forall y \in \R$ with $y > x.$ Show that $g \circ f$ is

convex.
\begin{align*}
(g \circ f)(x + t(y-x)) &= g(f(x + t(y-x))) \\
&\leq g(f(x) + t(f(y)-f(x))) \\
\end{align*}

\end{enumerate}
